\documentclass{article}
\begin{document}

\section{Normalization}

\large$$((\lambda a.(\lambda  b.b\ b)\ (\lambda b.b\ b))\ b)\ ((\lambda c.(c\ b))\ (\lambda a.a)) \rightarrow_\beta
((\lambda a.(\lambda  b.b\ b)\ (\lambda b.b\ b))\ b)\ ((\lambda a.a)\ b) \rightarrow_\beta$$
$$((\lambda a.(\lambda  b.b\ b)\ (\lambda b.b\ b))\ b)\ b \rightarrow_\beta
((\lambda  b.b\ b)\ (\lambda b.b\ b))\ b$$

\section{$S\ S\ K = I$}
$$S\ K\ K\ x =  (\lambda x\ y\ z.x\ z\ (y\ z)) (\lambda x\ y.x) (\lambda x\ y.x)\ x = (\lambda x\ y.x)\ x\ (\lambda y.x) = x => S K K = I$$

\end{document}
